# Lambda Calculus - Reductions #1
 
Reduce the following expression to no more than one term. If the expression cannot be reduced, enter "CAN'T REDUCE".

    ((λx.(x y))(λz.z))
Your answer should look like:

    u
(This is not the actual answer, just a demonstration of how you should present it.)

[Lambda Calculus Tutorial](http://www.inf.fu-berlin.de/inst/ag-ki/rojas_home/documents/tutorials/lambda.pdf)
## Explanation

    ((λx.(x y))(λz.z))

    = (λx.(x y))(λz.z)
    = ((λz.z)y)
    = (λz.z)y
    = y

## Code
```haskell
y
```