# Lambda Calculus - Reductions #2

Reduce the following to no more than **one term**. If the expression cannot be reduced, enter "CAN'T REDUCE".

    ((λx.((λy.(x y))x))(λz.w))
Your answer should look like:

    u
(This is not the actual answer, just a demonstration of how you should present it.)

## Explanation

    ((λx.((λy.(x y))x))(λz.w))
    = ((λx.((x x)))(λz.w))              -- replace y with variable x
    = (λz.w))                           -- replace x with variable x
    = w                                 -- replace z with variable w

## Code

```haskell
w
```