# Lambda Calculus - Reductions #4

Reduce the following expression, using the beta-rule, to no more than **one term**. If the expression cannot be reduced, enter "CAN'T REDUCE".

    (λg.((λf.((λx.(f (x x)))(λx.(f (x x))))) g)) 
Your answer should look like:

    u
(This is not the actual answer, just a demonstration of how you should present it.)

## Explanation

    (λg.((λf.((λx.(f (x x)))(λx.(f (x x))))) g)) 
    = (λg.((λf.((λx.(f (x x))))) g)) 
    = (λg.((λf.()) g)) 
    = (λg.((λf.) g)) 
    = (λg.g)) 
    = CAN'T REDUCE

## Code

```haskell
CAN'T REDUCE
```